

Definition 7

$n \in \mathbb{N}$ is odd if $(\exists i \in \mathbb{N}) n = 2i + 1$.

Proposition 8

Goal: $(\forall m, n \in \mathbb{N}) m \text{ and } n \text{ odd} \implies m \times n \text{ odd}$

Proof

Assume:

1. $m, n \in \mathbb{N}$
2. m and n odd

New goal: $m \times n$ odd

$$\begin{aligned}
 & (\exists i, j \in \mathbb{N}) m = 2i + 1 \wedge n = 2j + 1 \\
 \implies & (\exists i, j \in \mathbb{N}) m \times n = (2i + 1) \times (2j + 1) \\
 \implies & (\exists i, j \in \mathbb{N}) m \times n = 2(2ij + i + j) + 1 \\
 \implies & (\exists k \in \mathbb{N}) m \times n = 2k + 1 \\
 \implies & m \times n \text{ odd}
 \end{aligned}$$

Definition 9

$(\forall x \in \mathbb{R})$

- $(\exists m, n \in \mathbb{Z}) x = m/n \iff x \text{ rational}$
- $\neg(x \text{ rational}) \iff x \text{ irrational}$
- $x > 0 \iff x \text{ positive}$
- $x < 0 \iff x \text{ negative}$
- $\neg(x \text{ positive}) \iff x \text{ nonpositive}$
- $\neg(x \text{ negative}) \iff x \text{ nonnegative}$
- $x \text{ nonnegative} \wedge x \in \mathbb{Z} \iff x \in \mathbb{N}$

Proposition 10

Goal: $(\forall x \text{ positive}) \sqrt{x} \text{ rational} \implies x \text{ rational}$

Proof

Assume:

1. x positive
2. \sqrt{x} rational

New goal: x rational

$$\begin{aligned}
 & (\exists p, q \in \mathbb{Z}) \sqrt{x} = p/q \\
 \implies & (\exists p, q \in \mathbb{Z}) x = (\sqrt{x})^2 = p^2/q^2 \\
 \implies & (\exists p', q' \in \mathbb{Z}) x = p'/q' \\
 \iff & x \text{ rational}
 \end{aligned}$$

Definition

$$P \wedge (P \implies Q) \implies Q$$

Theorem 11

Goal: Let P_1, P_2, P_3 be statements, $(P_1 \implies P_2 \wedge P_2 \implies P_3) \implies (P_1 \implies P_3)$

Proof

Assume:

1. $P_1 \implies P_2$
2. $P_2 \implies P_3$
3. P_1

New goal: P_3

$$\begin{aligned}
 &P_2 \text{ as (4) by (1) and (3)} \\
 &\implies P_3 \text{ by (2) and (4)}
 \end{aligned}$$

Definition

$$(P \iff Q) \iff (P \implies Q \wedge P \impliedby Q)$$

Definition 12

$$d|n \iff (\exists k \in \mathbb{Z}) \ n = k \times d$$

Definition 14

$$(\forall m \in \mathbb{Z}^+, a, b \in \mathbb{Z}) \ a \equiv b \pmod{m} \iff m|(a - b)$$

Proposition 16

$$\text{Goal: } (n \text{ even} \iff n \equiv 0 \pmod{2}) \wedge (n \text{ odd} \iff n \equiv 1 \pmod{2})$$

Subgoal: $n \text{ even} \iff n \equiv 0 \pmod{2}$

Assume:

1. $n \text{ even}$

New goal: $n \equiv 0 \pmod{2}$

$$\begin{aligned}
 n \text{ even} &\iff (\exists k \in \mathbb{Z}) \ n = 2 \times k \\
 &\iff (\exists k \in \mathbb{Z}) \ (n - 0) = 2 \times k \\
 &\iff n \equiv 0 \pmod{2}
 \end{aligned}$$

Subgoal: $n \text{ odd} \iff n \equiv 1 \pmod{2}$

Assume:

1. $n \text{ odd}$

New goal: $n \equiv 1 \pmod{2}$

$$\begin{aligned}
 n \text{ odd} &\iff (\exists k \in \mathbb{Z}) \ n = 2 \times k + 1 \\
 &\iff (\exists k \in \mathbb{Z}) \ (n - 1) = 2 \times k \\
 &\iff n \equiv 1 \pmod{2}
 \end{aligned}$$

Proposition 18

$$\text{Goal: } (\forall m \in \mathbb{Z}^+, a, b \in \mathbb{Z}) \ a \equiv b \pmod{m} \iff ((\forall n \in \mathbb{Z}^+) \ n \times a \equiv n \times b \pmod{n \times m})$$

Assume:

1. $m \in \mathbb{Z}^+$
2. $a, b \in \mathbb{Z}$

Subgoal: $a \equiv b \pmod{m} \implies (\forall n \in \mathbb{Z}^+) n \times a \equiv n \times b \pmod{n \times m}$

Assume:

3. $a \equiv b \pmod{m}$

4. $n \in \mathbb{Z}^+$

New goal: $n \times a \equiv n \times b \pmod{n \times m}$

$$\begin{aligned} & (\exists i \in \mathbb{Z}) a - b = m \times i \text{ by (3)} \\ \implies & (\exists i \in \mathbb{Z}) n \times a - n \times b = (n \times m) \times i \\ \implies & (\exists i \in \mathbb{Z}) n \times a \equiv n \times b \pmod{n \times m} \\ \implies & n \times a \equiv n \times b \pmod{n \times m} \end{aligned}$$

Subgoal: $(\forall n \in \mathbb{Z}^+) n \times a \equiv n \times b \pmod{n \times m} \implies a \equiv b \pmod{m}$

Assume:

3. $(\forall n \in \mathbb{Z}^+) n \times a \equiv n \times b \pmod{n \times m}$

$$\begin{aligned} & 1 \times a \equiv 1 \times b \pmod{1 \times m} \text{ by (3)} \\ \implies & a \equiv b \pmod{m} \end{aligned}$$

Definition

- $(\forall x) x = x$
- $(\forall x, y) x = y \implies (P(x) \implies P(y))$
- $(\forall a, b, c) (a = b \wedge b = c) \implies a = c$
- $(\forall a, b, x, y) (a = b \wedge x = y) \implies (a + x = b + x = b + y)$